Restore registry limit value.

src/dafny/beacon/attestations/AttestationsHelpers.dfy
@@ -41,6 +41,13 @@ module AttestationsHelpers {
     import opened Validators
 
     /**
+     *  Non deterministic conversion of aggregation bits to validator indices.
+     */
+    // function aggregationBitsToValidatorIndices(xb: AggregationBits): (s: set<ValidatorIndex>) 
+    //     ensures  |trueBitsCount(xb)| == |s|
+
+
+    /**
      *  The number of attestations for a pair of checkpoints.
      *  
      *  @param  xa  The known list of attestations (votes).
@@ -48,7 +55,7 @@ module AttestationsHelpers {
      *  @param  tgt A checkpoint.
      *  @returns    The number of votes for src --> tgt in `xa`.
      */
-    function method countAttestationsForLink(xa : seq<PendingAttestation>, src : CheckPoint, tgt: CheckPoint) : nat
+    function method countAttestationsForLink(xa : seq<PendingAttestation>, src : CheckPoint, tgt: CheckPoint): nat
         ensures countAttestationsForLink(xa, src, tgt) <= |xa|
         decreases xa
     {
@@ -57,7 +64,6 @@ module AttestationsHelpers {
         else 
             (if xa[0].data.source == src && xa[0].data.target == tgt then 
                 1
-
             else 
                 0
             ) + countAttestationsForLink(xa[1..], src, tgt)
@@ -71,15 +77,17 @@ module AttestationsHelpers {
      *  @param  tgt     The target checkpoint of the link.
      *  @returns        The set of validators's indices that vote for (src. tgt) in `xa`. 
      */
-     function collectValidatorsAttestatingForLink(xa : seq<PendingAttestation>, src : CheckPoint, tgt: CheckPoint) : set<ValidatorIndex>
+     function collectValidatorsAttestatingForLink(xa : seq<PendingAttestation>, src : CheckPoint, tgt: CheckPoint) : set<ValidatorInCommitteeIndex>
         ensures forall e :: e in collectValidatorsAttestatingForLink(xa, src, tgt) ==>
             e < MAX_VALIDATORS_PER_COMMITTEE
         ensures |collectValidatorsAttestatingForLink(xa, src, tgt)| <= MAX_VALIDATORS_PER_COMMITTEE
-        ensures forall v :: v in collectValidatorsAttestatingForLink(xa, src, tgt) ==>
+        ensures forall v :: 0 <= v < MAX_VALIDATORS_PER_COMMITTEE ==>
+            (v in collectValidatorsAttestatingForLink(xa, src, tgt) <==>
             exists a :: a in xa 
                 && a.data.source == src 
                 && a.data.target == tgt 
                 && a.aggregation_bits[v]
+            )
 
         decreases xa
     {
@@ -95,21 +103,54 @@ module AttestationsHelpers {
             ) + collectValidatorsAttestatingForLink(xa[1..], src, tgt)
     }
 
+    // function collectValidatorsAttestatingForLink2(xa : seq<PendingAttestation>, src : CheckPoint, tgt: CheckPoint) : set<ValidatorIndex>
+    //     //  the next ensure is redundant as the ValidatorIndex type captures it.
+    //     ensures forall e :: e in collectValidatorsAttestatingForLink2(xa, src, tgt) ==>
+    //         e < VALIDATOR_REGISTRY_LIMIT as nat
+    //     ensures |collectValidatorsAttestatingForLink2(xa, src, tgt)| <= VALIDATOR_REGISTRY_LIMIT as nat
+    //     ensures forall v :: 
+    //         v in collectValidatorsAttestatingForLink2(xa, src, tgt) <==>
+    //         exists a, i : ValidatorInCommitteeIndex :: a in xa 
+    //             && a.data.source == src 
+    //             && a.data.target == tgt 
+    //             && a.aggregation_bits[i]
+    //             && a.aggregation_validators[i] == v 
+
+    //     decreases xa
+    // {
+    //     if |xa| == 0 then 
+    //         { }
+    //     else 
+    //         //
+    //         unionCardBound(
+    //             trueBitsCollect(xa[0].aggregation_bits, xa[0].aggregation_validators),
+    //             collectValidatorsAttestatingForLink2(xa[1..], src, tgt), 
+    //             VALIDATOR_REGISTRY_LIMIT as nat);
+    //         (if xa[0].data.source == src && xa[0].data.target == tgt then 
+    //             trueBitsCollect(xa[0].aggregation_bits, xa[0].aggregation_validators)
+    //             // trueBitsCount(xa[0].aggregation_bits)
+    //         else 
+    //             {}
+    //         ) + collectValidatorsAttestatingForLink2(xa[1..], src, tgt)
+    // }
+
     /**
      *  Collect set of indices of validators attesting a link to a given target.
      *
      *  @param  xa      A seq of attestations.
      *  @param  tgt     The target checkpoint of the link.
-     *  @returns        The set of validators's indices that vote for (_. tgt) in `xa`. 
+     *  @returns        The set of validators's indices that vote for (_.tgt) in `xa`. 
      */
-    function collectValidatorsIndicesAttestatingForTarget(xa : seq<PendingAttestation>, tgt: CheckPoint) : set<ValidatorIndex>
+    function collectValidatorsIndicesAttestatingForTarget(xa : seq<PendingAttestation>, tgt: CheckPoint) : set<ValidatorInCommitteeIndex>
         ensures forall e :: e in collectValidatorsIndicesAttestatingForTarget(xa, tgt) ==>
-            e < MAX_VALIDATORS_PER_COMMITTEE
+            0 <= e < MAX_VALIDATORS_PER_COMMITTEE
         ensures |collectValidatorsIndicesAttestatingForTarget(xa, tgt)| <= MAX_VALIDATORS_PER_COMMITTEE
-        ensures forall v :: v in collectValidatorsIndicesAttestatingForTarget(xa, tgt) ==>
+        ensures forall v :: 0 <= v < MAX_VALIDATORS_PER_COMMITTEE ==> 
+            (v in collectValidatorsIndicesAttestatingForTarget(xa, tgt) <==>
             exists a :: a in xa 
                 && a.data.target == tgt 
-                && a.aggregation_bits[v]       
+                && a.aggregation_bits[v]   
+            )    
         decreases xa
     {
         if |xa| == 0 then 
@@ -118,17 +159,43 @@ module AttestationsHelpers {
             unionCardBound(trueBitsCount(xa[0].aggregation_bits),
                 collectValidatorsIndicesAttestatingForTarget(xa[1..], tgt), MAX_VALIDATORS_PER_COMMITTEE);
             (if xa[0].data.target == tgt then 
+                //  Set of indices that are true in xa[0].aggregation_bits
                 trueBitsCount(xa[0].aggregation_bits)
             else 
                 {}
             ) + collectValidatorsIndicesAttestatingForTarget(xa[1..], tgt)
     }
 
+    // function collectValidatorsIndicesAttestatingForTarget2(xa : seq<PendingAttestation>, tgt: CheckPoint) : set<ValidatorIndex>
+    //     ensures forall e :: e in collectValidatorsIndicesAttestatingForTarget2(xa, tgt) ==>
+    //         e < VALIDATOR_REGISTRY_LIMIT as nat 
+    //     ensures |collectValidatorsIndicesAttestatingForTarget2(xa, tgt)| <= VALIDATOR_REGISTRY_LIMIT as nat 
+    //     ensures forall v :: 
+    //         v in collectValidatorsIndicesAttestatingForTarget2(xa, tgt) <==>
+    //         exists a, i : ValidatorInCommitteeIndex :: a in xa 
+    //             && a.data.target == tgt 
+    //             && a.aggregation_bits[i]
+    //             && a.aggregation_validators[i] == v 
+        // decreases xa
+    // {
+    //     if |xa| == 0 then 
+    //         { }
+    //     else 
+    //         unionCardBound(trueBitsCount(xa[0].aggregation_bits),
+    //             collectValidatorsIndicesAttestatingForTarget(xa[1..], tgt), MAX_VALIDATORS_PER_COMMITTEE);
+    //         (if xa[0].data.target == tgt then 
+    //             //  Set of indices that are true in xa[0].aggregation_bits
+    //             trueBitsCount(xa[0].aggregation_bits)
+    //         else 
+    //             {}
+    //         ) + collectValidatorsIndicesAttestatingForTarget(xa[1..], tgt)
+    // }
+
     /**
      *  Collect the set of indices for which xb[i] is true.
      *  
-     *  @param  xb  A sequence of bools.
-     *  @returns    The number of elements that are true in `xb`.
+     *  @param      xb  A sequence of bools.
+     *  @returns        The set of indices that are true in `xb`.
      */
     function trueBitsCount(xb : seq<bool>) : set<nat> 
         ensures |trueBitsCount(xb)| <= |xb|
@@ -140,6 +207,22 @@ module AttestationsHelpers {
         else 
             (if xb[|xb| - 1] then { |xb| - 1 } else {}) + trueBitsCount(xb[..|xb| - 1])
     }
+
+    //  function trueBitsCollect(xb : seq<bool>, xv: seq<ValidatorIndex>) : set<ValidatorIndex> 
+    //     requires |xb| == |xv|
+    //     ensures |trueBitsCollect(xb, xv)| <= |xb| == MAX_VALIDATORS_PER_COMMITTEE
+    //     ensures forall v :: v in trueBitsCollect(xb, xv) <==> 
+    //         exists k ::  0 <= k < |xb| 
+    //             && xb[k]
+    //             && xv[k] == v 
+        // decreases xb
+    // {
+    //     if |xb| == 0 then 
+    //         {}
+    //     else 
+    //         (if xb[|xb| - 1] then { |xb| - 1 } else {}) 
+    //         + trueBitsCollect(xb[..|xb| - 1])
+    // }
 
     /**
      *  The set of validators attesting to a target is larger than the set 
